wip

example_userbase.thy
@@ -39,14 +39,52 @@ definition lsInit :: "localState" where
   querySpec :: "operation \<Rightarrow> 'any list \<Rightarrow> 'any operationContext \<Rightarrow> 'any \<Rightarrow> bool"
   procedure :: "procedureName \<Rightarrow> 'any list \<rightharpoonup> ('localState \<times> ('localState, 'any) procedureImpl)"
   invariant :: "'any invariantContext \<Rightarrow> bool"
-*)  
+*)
+
+(* define used names, to avoid typos and to help Isabelle*)
+
+definition "users_name_assign \<equiv> ''users_name_assign''"
+definition "users_mail_assign \<equiv> ''users_mail_assign''"
+definition "users_contains_key \<equiv> ''users_contains_key''"
+definition "users_remove \<equiv> ''users_remove''"
+definition "users_name_get \<equiv> ''users_name_get''"
+definition "users_mail_get \<equiv> ''users_mail_get''"
+definition "registerUser \<equiv> ''registerUser''"
+definition "updateMail \<equiv> ''updateMail''"
+definition "removeUser \<equiv> ''removeUser''"
+definition "getUser \<equiv> ''getUser''"
+
+lemma names_distinct: "distinct [users_name_assign, users_mail_assign, users_contains_key, users_remove, users_name_get, users_mail_get, registerUser, updateMail, removeUser, getUser]"
+  by eval
+
+lemma distinct_perm1: "distinct [x,y] \<longleftrightarrow> x \<noteq> y \<and> y \<noteq> x"
+  by auto
+
+lemma distinct_perm2: "distinct (x#xs) \<longleftrightarrow> (\<forall>y\<in>set xs. x \<noteq> y \<and> y \<noteq> x) \<and> distinct xs"
+  by auto
+
+lemma distinct_perm3: "(\<forall>x\<in>set [x]. P x) \<longleftrightarrow> P x"
+  by auto
+
+lemma distinct_perm4: "(\<forall>x\<in>set (y#ys). P x) \<longleftrightarrow> (P y \<and> (\<forall>x\<in>set ys. P x))"
+  by auto
+
+schematic_goal name_distinct2: "?X"
+  apply (insert names_distinct)
+  apply (subst(asm) distinct_perm1 distinct_perm2)+
+  apply (subst(asm) distinct_perm3 distinct_perm4)+
+  apply assumption
+  done
+
+
+
 
 definition registerUserImpl :: "(localState, val) procedureImpl" where
 "registerUserImpl ls \<equiv> [
    (* 0 *) NewId (\<lambda>x. (ls\<lparr>ls_u := x, ls_pc := 1\<rparr> :: localState)),
    (* 1 *) BeginAtomic (ls\<lparr>ls_pc := 2\<rparr>),
-   (* 2 *) DbOperation ''users_name_assign'' [ls_u ls, String (ls_name ls)] (\<lambda>r. ls\<lparr>ls_pc := 3\<rparr>),
-   (* 3 *) DbOperation ''users_mail_assign'' [ls_u ls, String (ls_mail ls)] (\<lambda>r. ls\<lparr>ls_pc := 4\<rparr>),
+   (* 2 *) DbOperation users_name_assign [ls_u ls, String (ls_name ls)] (\<lambda>r. ls\<lparr>ls_pc := 3\<rparr>),
+   (* 3 *) DbOperation users_mail_assign [ls_u ls, String (ls_mail ls)] (\<lambda>r. ls\<lparr>ls_pc := 4\<rparr>),
    (* 4 *) EndAtomic (ls\<lparr>ls_pc := 5\<rparr>),
    (* 5 *) Return (ls_u ls)
    ] ! ls_pc ls"
@@ -54,9 +92,9 @@ definition registerUserImpl :: "(localState, val) procedureImpl" where
 definition updateMailImpl :: "(localState, val) procedureImpl" where
 "updateMailImpl ls \<equiv> [
    (* 0 *) BeginAtomic (ls\<lparr>ls_pc := 1\<rparr>),
-   (* 1 *) DbOperation ''users_contains_key'' [ls_u ls] (\<lambda>r. ls\<lparr>ls_exists := (r = Bool True), ls_pc := 2 \<rparr>),
+   (* 1 *) DbOperation users_contains_key [ls_u ls] (\<lambda>r. ls\<lparr>ls_exists := (r = Bool True), ls_pc := 2 \<rparr>),
    (* 2 *) LocalStep (if ls_exists ls then ls\<lparr>ls_pc := 3\<rparr> else ls\<lparr>ls_pc := 4\<rparr> ),
-   (* 3 *) DbOperation ''users_mail_assign'' [ls_u ls, String (ls_mail ls)] (\<lambda>r. ls\<lparr>ls_pc := 4\<rparr>),
+   (* 3 *) DbOperation users_mail_assign [ls_u ls, String (ls_mail ls)] (\<lambda>r. ls\<lparr>ls_pc := 4\<rparr>),
    (* 5 *) EndAtomic  (ls\<lparr>ls_pc := 6\<rparr>),
    (* 6 *) Return Undef
    ] ! ls_pc ls"   
@@ -64,18 +102,18 @@ definition updateMailImpl :: "(localState, val) procedureImpl" where
 definition removeUserImpl :: "(localState, val) procedureImpl" where
 "removeUserImpl ls \<equiv> [
    (* 0 *) BeginAtomic (ls\<lparr>ls_pc := 1\<rparr>),
-   (* 1 *) DbOperation ''users_remove'' [ls_u ls] (\<lambda>r. ls\<lparr>ls_pc := 2 \<rparr>),
+   (* 1 *) DbOperation users_remove [ls_u ls] (\<lambda>r. ls\<lparr>ls_pc := 2 \<rparr>),
    (* 2 *) EndAtomic  (ls\<lparr>ls_pc := 3\<rparr>),
    (* 3 *) Return Undef
-   ] ! ls_pc ls"      
+   ] ! ls_pc ls"
    
 definition getUserImpl :: "(localState, val) procedureImpl" where
 "getUserImpl ls \<equiv> [
    (* 0 *) BeginAtomic (ls\<lparr>ls_pc := 1\<rparr>),
-   (* 1 *) DbOperation ''users_contains_key'' [ls_u ls] (\<lambda>r. ls\<lparr>ls_exists := (r = Bool True), ls_pc := 2 \<rparr>),
+   (* 1 *) DbOperation users_contains_key [ls_u ls] (\<lambda>r. ls\<lparr>ls_exists := (r = Bool True), ls_pc := 2 \<rparr>),
    (* 2 *) LocalStep (if ls_exists ls then ls\<lparr>ls_pc := 3\<rparr> else ls\<lparr>ls_pc := 5\<rparr> ),
-   (* 3 *) DbOperation ''users_name_get'' [ls_u ls] (\<lambda>r. ls\<lparr>ls_name := stringval r, ls_pc := 4 \<rparr>),
-   (* 4 *) DbOperation ''users_mail_get'' [ls_u ls] (\<lambda>r. ls\<lparr>ls_mail := stringval r, ls_pc := 5 \<rparr>),
+   (* 3 *) DbOperation users_name_get [ls_u ls] (\<lambda>r. ls\<lparr>ls_name := stringval r, ls_pc := 4 \<rparr>),
+   (* 4 *) DbOperation users_mail_get [ls_u ls] (\<lambda>r. ls\<lparr>ls_mail := stringval r, ls_pc := 5 \<rparr>),
    (* 5 *) EndAtomic  (ls\<lparr>ls_pc := 6\<rparr>),
    (* 6 *) Return (if ls_exists ls then Found (ls_name ls) (ls_mail ls) else NotFound )
    ] ! ls_pc ls"      
@@ -83,22 +121,22 @@ definition getUserImpl :: "(localState, val) procedureImpl" where
    
 definition procedures where
 "procedures proc args \<equiv> 
-  if proc = ''registerUser'' then
+  if proc = registerUser then
     case args of 
       [String name, String mail] \<Rightarrow> 
         Some (lsInit\<lparr>ls_name := name, ls_mail := mail \<rparr> , registerUserImpl)
       | _ \<Rightarrow> None
-  else if proc = ''updateMail'' then 
+  else if proc = updateMail then 
     case args of 
       [UserId u, String mail] \<Rightarrow> 
         Some (lsInit\<lparr>ls_u := UserId u, ls_mail := mail \<rparr> , updateMailImpl)
       | _ \<Rightarrow> None
-  else if proc = ''removeUser'' then 
+  else if proc = removeUser then 
     case args of 
       [UserId u] \<Rightarrow> 
         Some (lsInit\<lparr>ls_u := UserId u \<rparr> , removeUserImpl)
       | _ \<Rightarrow> None
-  else if proc = ''getUser'' then 
+  else if proc = getUser then 
     case args of 
       [UserId u] \<Rightarrow> 
         Some (lsInit\<lparr>ls_u := UserId u \<rparr> , getUserImpl)
@@ -109,31 +147,31 @@ definition procedures where
 
 definition latest_name_assign :: "val operationContext \<Rightarrow> val \<Rightarrow> val set" where
 "latest_name_assign ctxt u \<equiv>  {v | c1 v. 
-     calls ctxt c1 \<triangleq> Call ''users_name_assign'' [u, v] Undef
-   \<and> (\<forall>c2. calls ctxt c2 \<triangleq> Call ''users_remove'' [u] Undef \<longrightarrow> (c2,c1)\<in>happensBefore ctxt)
-   \<and> (\<forall>c2 v'. calls ctxt c2 \<triangleq> Call ''users_name_assign'' [u] v' \<longrightarrow> \<not>(c1,c2)\<in>happensBefore ctxt)}"
+     calls ctxt c1 \<triangleq> Call users_name_assign [u, v] Undef
+   \<and> (\<forall>c2. calls ctxt c2 \<triangleq> Call users_remove [u] Undef \<longrightarrow> (c2,c1)\<in>happensBefore ctxt)
+   \<and> (\<forall>c2 v'. calls ctxt c2 \<triangleq> Call users_name_assign [u] v' \<longrightarrow> \<not>(c1,c2)\<in>happensBefore ctxt)}"
 
 definition latest_mail_assign :: "val operationContext \<Rightarrow> val \<Rightarrow> val set" where
 "latest_mail_assign ctxt u \<equiv>  {v | c1 v. 
-     calls ctxt c1 \<triangleq> Call ''users_mail_assign'' [u, v] Undef
-   \<and> (\<forall>c2. calls ctxt c2 \<triangleq> Call ''users_remove'' [u] Undef \<longrightarrow> (c2,c1)\<in>happensBefore ctxt)
-   \<and> (\<forall>c2 v'. calls ctxt c2 \<triangleq> Call ''users_mail_assign'' [u] v' \<longrightarrow> \<not>(c1,c2)\<in>happensBefore ctxt)}"   
+     calls ctxt c1 \<triangleq> Call users_mail_assign [u, v] Undef
+   \<and> (\<forall>c2. calls ctxt c2 \<triangleq> Call users_remove [u] Undef \<longrightarrow> (c2,c1)\<in>happensBefore ctxt)
+   \<and> (\<forall>c2 v'. calls ctxt c2 \<triangleq> Call users_mail_assign [u] v' \<longrightarrow> \<not>(c1,c2)\<in>happensBefore ctxt)}"   
    
 definition crdtSpec :: "operation \<Rightarrow> val list \<Rightarrow> val operationContext \<Rightarrow> val \<Rightarrow> bool" where
 "crdtSpec oper args ctxt res \<equiv> 
-  if oper \<in> {''users_name_assign'', ''users_mail_assign'', ''users_remove''} then
+  if oper \<in> {users_name_assign, users_mail_assign, users_remove} then
     (* update-operations always return Undef *)
     res = Undef
-  else if oper = ''users_contains_key'' then
-    res = Bool (\<exists>c1 v. (calls ctxt c1 \<triangleq> Call ''users_name_assign'' (args @ [v]) Undef
-                 \<or> calls ctxt c1 \<triangleq> Call ''users_mail_assign'' (args @ [v]) Undef)
-               \<and> (\<forall>c2. calls ctxt c2 \<triangleq> Call ''users_remove'' args Undef \<longrightarrow> (c2,c1)\<in>happensBefore ctxt))
-  else if oper = ''users_name_get'' then 
+  else if oper = users_contains_key then
+    res = Bool (\<exists>c1 v. (calls ctxt c1 \<triangleq> Call users_name_assign (args @ [v]) Undef
+                 \<or> calls ctxt c1 \<triangleq> Call users_mail_assign (args @ [v]) Undef)
+               \<and> (\<forall>c2. calls ctxt c2 \<triangleq> Call users_remove args Undef \<longrightarrow> (c2,c1)\<in>happensBefore ctxt))
+  else if oper = users_name_get then 
     if latest_name_assign ctxt (hd args) = {} then 
       res = Undef
     else
       res \<in> latest_name_assign ctxt (hd args)
-  else if oper = ''users_mail_get'' then 
+  else if oper = users_mail_get then 
     if latest_mail_assign ctxt (hd args) = {} then 
       res = Undef
     else
@@ -143,22 +181,22 @@ definition crdtSpec :: "operation \<Rightarrow> val list \<Rightarrow> val opera
   
 definition inv1 :: "val invariantContext \<Rightarrow> bool" where
 "inv1 ctxt \<equiv> \<forall>r g u.
-    i_invocationOp ctxt r \<triangleq> (''removeUser'', [u])
-  \<and> i_invocationOp ctxt g \<triangleq> (''getUser'', [u])
+    i_invocationOp ctxt r \<triangleq> (removeUser, [u])
+  \<and> i_invocationOp ctxt g \<triangleq> (getUser, [u])
   \<and> (r,g) \<in> invocation_happensBefore ctxt
   \<longrightarrow> i_invocationRes ctxt g \<triangleq> NotFound"
   
 definition inv2 :: "val invariantContext \<Rightarrow> bool" where
 "inv2 ctxt \<equiv> \<forall>u i.
-    i_invocationOp ctxt i \<triangleq> (''removeUser'', [u])
+    i_invocationOp ctxt i \<triangleq> (removeUser, [u])
   \<and> i_invocationRes ctxt i \<noteq> None
-  \<longrightarrow> (\<exists>c. i_callOriginI ctxt c \<triangleq> i \<and> calls ctxt c \<triangleq> Call ''users_remove'' [u] Undef)"
+  \<longrightarrow> (\<exists>c. i_callOriginI ctxt c \<triangleq> i \<and> calls ctxt c \<triangleq> Call users_remove [u] Undef)"
   
 definition inv3 :: "val invariantContext \<Rightarrow> bool" where
 "inv3 ctxt \<equiv> \<not>(\<exists>write delete u v.
-  (calls ctxt write \<triangleq> Call ''users_name_assign'' [u, v] Undef
-    \<or> calls ctxt write \<triangleq> Call ''users_mail_assign'' [u, v] Undef)
-  \<and> (calls ctxt delete \<triangleq> Call ''users_remove'' [u] Undef)
+  (calls ctxt write \<triangleq> Call users_name_assign [u, v] Undef
+    \<or> calls ctxt write \<triangleq> Call users_mail_assign [u, v] Undef)
+  \<and> (calls ctxt delete \<triangleq> Call users_remove [u] Undef)
   \<and> (delete, write) \<in> happensBefore ctxt
   )"
   
@@ -172,18 +210,86 @@ definition progr :: "(localState, val) prog" where
   invariant = inv
 \<rparr>"
 
+lemma procedure_progr[simp]: "procedure progr = procedures"
+  by (simp add: progr_def)
+
+
+lemma if_split_h: "\<lbrakk>c \<Longrightarrow> P x; \<not>c \<Longrightarrow> P y\<rbrakk>  \<Longrightarrow> P (if c then x else y)"
+  by auto
+
+lemma procedure_cases: "procedures procName args \<noteq> None \<Longrightarrow> procName \<in> {registerUser, updateMail, removeUser, getUser}"
+  by (auto simp add: procedures_def split: if_splits)
+
+lemma procedure_cases': "\<lbrakk>procedures procName args \<triangleq> x; procName \<noteq> registerUser; procName \<noteq> updateMail; procName \<noteq> removeUser\<rbrakk> \<Longrightarrow> procName = getUser"
+  by (auto simp add: procedures_def split: if_splits)
+
+lemma procedure_case_split: "\<lbrakk>procedures procName args \<triangleq> x; procName = registerUser \<Longrightarrow> P; procName = updateMail \<Longrightarrow> P; procName = removeUser \<Longrightarrow> P; procName = getUser \<Longrightarrow> P\<rbrakk> \<Longrightarrow> P"
+  using procedure_cases' by blast
+
+
+lemma procedure_cases2: "procedures procName args \<triangleq> (initState, impl) \<longleftrightarrow> (
+  (\<exists>name mail. procName = registerUser \<and> args = [String name, String mail] \<and> initState = lsInit\<lparr>ls_name := name, ls_mail := mail \<rparr> \<and> impl = registerUserImpl)
+\<or> (\<exists>u mail. procName = updateMail \<and> args = [UserId u, String mail] \<and> initState = lsInit\<lparr>ls_u := UserId u, ls_mail := mail \<rparr> \<and> impl = updateMailImpl)
+\<or> (\<exists>u. procName = removeUser \<and> args = [UserId u] \<and> initState = lsInit\<lparr>ls_u := UserId u \<rparr> \<and> impl = removeUserImpl)
+\<or> (\<exists>u. procName = getUser \<and> args = [UserId u] \<and> initState = lsInit\<lparr>ls_u := UserId u \<rparr> \<and> impl = getUserImpl))" (is "?Left \<longleftrightarrow> ?Right")
+proof
+  assume a: ?Left
+
+  thm a
+  thm procedure_case_split[OF a]
+
+  show ?Right
+    apply (rule procedure_case_split[OF a])
+    apply (auto simp add:)
+        apply (rule a)
+    thm a
+
+
+
+  apply (auto simp add: dest: procedure_cases')
+  using procedure_cases' apply blast
+
+
+
+
+
+
+proof 
+
+  from procedure_cases
+  have "procName \<in> {registerUser'', ''updateMail'', ''removeUser'', ''getUser}"
+
+
+
+  apply standard
+  apply auto[1]
+
+  apply (subst procedure_progr)
+  apply (subst procedures_def)
+  apply (rule if_cases)
+  apply (auto split: list.splits)[1]
+  apply (rule if_split_h, clarsimp split: list.splits)+
+  
+  done
+
 
 theorem "programCorrect progr"
-proof (rule show_correctness_via_single_session)
+proof (rule show_programCorrect_using_checkCorrect)
   have [simp]: "invariant progr = inv" by (simp add: progr_def)
 
   have [simp]: "S \<in> initialStates progr i \<Longrightarrow> prog S = progr" for S i
     by (auto simp add: initialStates_def)
   
-  show "invariant_all (replissSem1.initialState progr)"
-     by (auto simp add: initialState_def invariant_all_def inv_def inv1_def inv2_def inv3_def invContextH_def)
+  show "invariant_all (repliss_sem.initialState progr)"
+     by (auto simp add: initialState_def  inv_def inv1_def inv2_def inv3_def invContextH_def)
   
-     
+   show "\<And>S i. S \<in> initialStates progr i \<Longrightarrow> invariant_all S"
+     apply (subst(asm) initialStates_def)
+     apply auto
+
+     apply (auto simp add: initialState_def  inv_def inv1_def inv2_def inv3_def invContextH_def)
+
+
      
   show "programCorrect_s progr"
   proof (rule show_program_correct_single_invocation)
